Review Raw RSA Keyring and fix Indexing bug in RawRSAKeyring (#69, #75)
With this change, we review the work done on the Raw RSA Keyring and edit a known indexing bug.
This change does not review the work done on  RSAEncryption (solely the RawRSAKeyring).
Additionally, this change does not prevent future indexing bugs from occurring. Preventing these will occur after additional team discussions.

Verified with dafny and successful unit tests.

src/extern/dotnet/RSAEncryption.cs
@@ -90,7 +90,7 @@ namespace RSAEncryption {
                 } else if (padding.is_OAEP__SHA1) {
                     engine = new OaepEncoding(new RsaEngine(), new Sha1Digest(), null);
                 }
-                else { // paddingi_is_OAEP__SHA256
+                else { // padding._is_OAEP__SHA256
                     engine = new OaepEncoding(new RsaEngine(), new Sha256Digest(), null);
                 }
 
